rename + reorganize

Bachmair_Ganzinger/New2_FO_Resolution_Prover.thy
@@ -52,23 +52,6 @@ context
 begin
 
 (* Move to substitution maybe:*)
-definition subst_atm_list :: "'a list \<Rightarrow> 's \<Rightarrow> 'a list" (infixl "\<cdot>al" 67) where
-  "As \<cdot>al \<sigma> = map (\<lambda>A. A \<cdot>a \<sigma>) As"
-  
-lemma subst_atm_lst_id_subst[simp]: "As \<cdot>al id_subst = As"
-  unfolding subst_atm_list_def by auto
-
-definition subst_mcls :: "'a main_clause \<Rightarrow> 's \<Rightarrow> 'a main_clause" (infixl "\<cdot>amc" 67) where
-  "DAs \<cdot>amc \<sigma> = (get_C DAs \<cdot> \<sigma>, get_As DAs \<cdot>al \<sigma>)"
-  
-lemma subst_mcl_id_subst[simp]: "DAs \<cdot>amc id_subst = DAs"
-  unfolding subst_mcls_def by auto
-
-definition subst_scls :: "'a side_clause \<Rightarrow> 's \<Rightarrow> 'a side_clause" (infixl "\<cdot>sc" 67) where
-  "CAs \<cdot>sc \<sigma> = (get_C CAs \<cdot> \<sigma>, get_As CAs \<cdot>am \<sigma>)"
-  
-lemma subst_scl_id_subst[simp]: "CAs \<cdot>sc id_subst = CAs"
-  unfolding subst_scls_def by auto
   
 abbreviation "maximal_in A DAs \<equiv> (\<forall>B \<in> atms_of DAs. \<not> less_atm A B)"
   (* This definition is a bit inconsistent compared to the ground case since 
@@ -108,7 +91,7 @@ inductive ord_resolve_rename :: "'a side_clause list \<Rightarrow> 'a main_claus
   "is_renaming \<rho> \<Longrightarrow>
    (\<forall>\<rho> \<in> set P. is_renaming \<rho>) \<Longrightarrow>
    length P = length CAs \<Longrightarrow>
-   ord_resolve (map (\<lambda>(C,\<rho>). C \<cdot>sc \<rho>) (zip CAs P)) (DAs \<cdot>amc \<rho>) E \<Longrightarrow>
+   ord_resolve (map (\<lambda>(C,\<rho>). C \<cdot>sc \<rho>) (zip CAs P)) (DAs \<cdot>mc \<rho>) E \<Longrightarrow>
    ord_resolve_rename CAs DAs E"
   (* In this definition, P, \<sigma> and \<rho>, are not part of the signature. 
      A bit different from ord_resolve... *)
